Rename example prefix in 'Test.ReduceTactics'

He4/Language/Test/ReduceTactics.v
@@ -16,123 +16,123 @@ Section Examples.
 Open Scope oo_scope.
 Open Scope state_scope.
 
-Definition ex_reduce_tnot_tm := !!tbool true.
-Example ex_reduce_tnot:
+Definition ex_tnot_tm := !!tbool true.
+Example ex_tnot:
   forall st,
-  ex_reduce_tnot_tm / st ==>* tbool true / st.
+  ex_tnot_tm / st ==>* tbool true / st.
 Proof.
-  unfold ex_reduce_tnot_tm. intros. repeat reduce. Qed.
+  unfold ex_tnot_tm. intros. repeat reduce. Qed.
 
-Definition ex_reduce_tand_tm := !tbool false \&& !tbool true \&& tbool true.
-Example ex_reduce_tand:
+Definition ex_tand_tm := !tbool false \&& !tbool true \&& tbool true.
+Example ex_tand:
   forall st,
-  ex_reduce_tand_tm / st ==>* tbool false / st.
+  ex_tand_tm / st ==>* tbool false / st.
 Proof.
-  unfold ex_reduce_tand_tm. intros. repeat reduce. Qed.
+  unfold ex_tand_tm. intros. repeat reduce. Qed.
 
-Definition ex_reduce_tor_tm := !tbool true \|| !tbool false \|| tbool false.
-Example ex_reduce_tor:
+Definition ex_tor_tm := !tbool true \|| !tbool false \|| tbool false.
+Example ex_tor:
   forall st,
-  ex_reduce_tor_tm / st ==>* tbool true / st.
+  ex_tor_tm / st ==>* tbool true / st.
 Proof.
-  unfold ex_reduce_tor_tm. intros. repeat reduce. Qed.
+  unfold ex_tor_tm. intros. repeat reduce. Qed.
 
-Definition ex_reduce_tplus_tm := (tnat 3 \+ tnat 4) \+ (tnat 5 \+ tnat 6).
-Example ex_reduce_tplus:
+Definition ex_tplus_tm := (tnat 3 \+ tnat 4) \+ (tnat 5 \+ tnat 6).
+Example ex_tplus:
   forall st,
-  ex_reduce_tplus_tm / st ==>* tnat 18 / st.
+  ex_tplus_tm / st ==>* tnat 18 / st.
 Proof.
-  unfold ex_reduce_tplus_tm. intros. repeat reduce. Qed.
+  unfold ex_tplus_tm. intros. repeat reduce. Qed.
 
-Definition ex_reduce_tminus_tm := (tnat 3 \+ tnat 4) \- (tnat 1 \+ tnat 2).
-Example ex_reduce_tminus:
+Definition ex_tminus_tm := (tnat 3 \+ tnat 4) \- (tnat 1 \+ tnat 2).
+Example ex_tminus:
   forall st,
-  ex_reduce_tminus_tm / st ==>* tnat 4 / st.
+  ex_tminus_tm / st ==>* tnat 4 / st.
 Proof.
-  unfold ex_reduce_tminus_tm. intros. repeat reduce. Qed.
+  unfold ex_tminus_tm. intros. repeat reduce. Qed.
 
-Definition ex_reduce_tmult_tm := (tnat 3 \+ tnat 4) \* (tnat 1 \+ tnat 2).
-Example ex_reduce_tmult:
+Definition ex_tmult_tm := (tnat 3 \+ tnat 4) \* (tnat 1 \+ tnat 2).
+Example ex_tmult:
   forall st,
-  ex_reduce_tmult_tm / st ==>* tnat 21 / st.
+  ex_tmult_tm / st ==>* tnat 21 / st.
 Proof.
-  unfold ex_reduce_tmult_tm. intros. repeat reduce. Qed.
+  unfold ex_tmult_tm. intros. repeat reduce. Qed.
 
-Definition ex_reduce_teq_tm_1 := !tbool true \== !tbool false.
-Example ex_reduce_teq_1:
+Definition ex_teq_tm_1 := !tbool true \== !tbool false.
+Example ex_teq_1:
   forall st,
-  ex_reduce_teq_tm_1 / st ==>* tbool false / st.
+  ex_teq_tm_1 / st ==>* tbool false / st.
 Proof.
-  unfold ex_reduce_teq_tm_1. intros. repeat reduce. Qed.
+  unfold ex_teq_tm_1. intros. repeat reduce. Qed.
 
-Definition ex_reduce_teq_tm_2 := tvoid \== tvoid.
-Example ex_reduce_teq_2:
+Definition ex_teq_tm_2 := tvoid \== tvoid.
+Example ex_teq_2:
   forall st,
-  ex_reduce_teq_tm_2 / st ==>* tbool true / st.
+  ex_teq_tm_2 / st ==>* tbool true / st.
 Proof.
-  unfold ex_reduce_teq_tm_2. intros. repeat reduce. Qed.
+  unfold ex_teq_tm_2. intros. repeat reduce. Qed.
 
-Definition ex_reduce_teq_tm_3 := tnat 0 \== tnat 0.
-Example ex_reduce_teq_3:
+Definition ex_teq_tm_3 := tnat 0 \== tnat 0.
+Example ex_teq_3:
   forall st,
-  ex_reduce_teq_tm_3 / st ==>* tbool true / st.
+  ex_teq_tm_3 / st ==>* tbool true / st.
 Proof.
-  unfold ex_reduce_teq_tm_3. intros. repeat reduce. Qed.
+  unfold ex_teq_tm_3. intros. repeat reduce. Qed.
 
-Definition ex_reduce_teq_tm_4 := tbool true \== tbool true.
-Example ex_reduce_teq_4:
+Definition ex_teq_tm_4 := tbool true \== tbool true.
+Example ex_teq_4:
   forall st,
-  ex_reduce_teq_tm_4 / st ==>* tbool true / st.
+  ex_teq_tm_4 / st ==>* tbool true / st.
 Proof.
-  unfold ex_reduce_teq_tm_4. intros. repeat reduce. Qed.
+  unfold ex_teq_tm_4. intros. repeat reduce. Qed.
 
-Definition ex_reduce_teq_tm_5 := tref 0 \== tref 0.
-Example ex_reduce_teq_5:
+Definition ex_teq_tm_5 := tref 0 \== tref 0.
+Example ex_teq_5:
   forall st,
-  ex_reduce_teq_tm_5 / st ==>* tbool true / st.
+  ex_teq_tm_5 / st ==>* tbool true / st.
 Proof.
-  unfold ex_reduce_teq_tm_5. intros. repeat reduce. Qed.
+  unfold ex_teq_tm_5. intros. repeat reduce. Qed.
 
-Definition ex_reduce_teq_tm_6 := trc (tbool true) tvoid \== trc (tbool true) tvoid.
-Example ex_reduce_teq_6:
+Definition ex_teq_tm_6 := trc (tbool true) tvoid \== trc (tbool true) tvoid.
+Example ex_teq_6:
   forall st,
-  ex_reduce_teq_tm_6 / st ==>* tbool true / st.
+  ex_teq_tm_6 / st ==>* tbool true / st.
 Proof.
-  unfold ex_reduce_teq_tm_6. intros. repeat reduce. Qed.
+  unfold ex_teq_tm_6. intros. repeat reduce. Qed.
 
-Definition ex_reduce_teq_tm_7 := tcl "Foo" tvoid \== tcl "Foo" tvoid.
-Example ex_reduce_teq_7:
+Definition ex_teq_tm_7 := tcl "Foo" tvoid \== tcl "Foo" tvoid.
+Example ex_teq_7:
   forall st,
-  ex_reduce_teq_tm_7 / st ==>* tbool true / st.
+  ex_teq_tm_7 / st ==>* tbool true / st.
 Proof.
-  unfold ex_reduce_teq_tm_7. intros. repeat reduce. Qed.
+  unfold ex_teq_tm_7. intros. repeat reduce. Qed.
 
-Definition ex_reduce_tvar_tm := tvar 0.
-Example ex_reduce_tvar:
+Definition ex_tvar_tm := tvar 0.
+Example ex_tvar:
   let st := write_sk_hd 0 (tbool true) (resize_sk_hd 1 init_state) in
-  ex_reduce_tvar_tm / st ==>* tbool true / st.
+  ex_tvar_tm / st ==>* tbool true / st.
 Proof.
-  unfold ex_reduce_tvar_tm. repeat reduce. Qed.
+  unfold ex_tvar_tm. repeat reduce. Qed.
 
-Definition ex_reduce_tassign_tm := tvar 0 ::= tnat 1 \+ tnat 1.
-Example ex_reduce_tassign:
+Definition ex_tassign_tm := tvar 0 ::= tnat 1 \+ tnat 1.
+Example ex_tassign:
   let st := resize_sk_hd 1 init_state in
   let st' := write_sk_hd 0 (tnat 2) st in
-  ex_reduce_tassign_tm / st ==>* tvoid / st'.
+  ex_tassign_tm / st ==>* tvoid / st'.
 Proof.
-  unfold ex_reduce_tassign_tm. repeat reduce. Qed.
+  unfold ex_tassign_tm. repeat reduce. Qed.
 
-Definition ex_reduce_tseq_tm :=
+Definition ex_tseq_tm :=
     tvar 0 ::= tnat 1 \+ tnat 1;
     tnat 3 \+ tvar 0.
-Example ex_reduce_tseq:
+Example ex_tseq:
   let st := resize_sk_hd 1 init_state in
   let st' := write_sk_hd 0 (tnat 2) st in
-  ex_reduce_tseq_tm / st ==>* tnat 5 / st'.
+  ex_tseq_tm / st ==>* tnat 5 / st'.
 Proof.
-  unfold ex_reduce_tseq_tm. repeat reduce. Qed.
+  unfold ex_tseq_tm. repeat reduce. Qed.
 
-Definition ex_reduce_tif_tm :=
+Definition ex_tif_tm :=
     \if !tbool true
     \then
       tnat 1
@@ -144,13 +144,13 @@ Definition ex_reduce_tif_tm :=
         tnat 3
       \fi
     \fi.
-Example ex_reduce_tif:
+Example ex_tif:
   forall st,
-  ex_reduce_tif_tm / st ==>* tnat 2 / st.
+  ex_tif_tm / st ==>* tnat 2 / st.
 Proof.
-  unfold ex_reduce_tif_tm. intros. repeat reduce. Qed.
+  unfold ex_tif_tm. intros. repeat reduce. Qed.
 
-Definition ex_reduce_twhile_tm :=
+Definition ex_twhile_tm :=
   let x := tvar 1 in
   let y := tvar 2 in
   (
@@ -162,84 +162,84 @@ Definition ex_reduce_twhile_tm :=
     \done;
     y
   ).
-Example ex_reduce_twhile:
+Example ex_twhile:
   let st := write_sk_hd 1 (tnat 3) (resize_sk_hd 3 init_state) in
   let st' := write_sk_hd 1 (tnat 0) (write_sk_hd 2 (tnat 6) st) in
-  ex_reduce_twhile_tm / st ==>* tnat 6 / st'.
+  ex_twhile_tm / st ==>* tnat 6 / st'.
 Proof.
-  unfold ex_reduce_twhile_tm. repeat reduce. Qed.
+  unfold ex_twhile_tm. repeat reduce. Qed.
 
-Definition ex_reduce_trc_tm := <(tnat 1 \+ tnat 2, tnat 3 \+ tnat 4)>.
-Example ex_reduce_trc:
+Definition ex_trc_tm := <(tnat 1 \+ tnat 2, tnat 3 \+ tnat 4)>.
+Example ex_trc:
   forall st,
-  ex_reduce_trc_tm / st ==>* <(tnat 3, tnat 7)> / st.
+  ex_trc_tm / st ==>* <(tnat 3, tnat 7)> / st.
 Proof.
-  unfold ex_reduce_trc_tm. intros. simpl. repeat reduce. Qed.
+  unfold ex_trc_tm. intros. simpl. repeat reduce. Qed.
 
-Definition ex_reduce_tcall_tm := tcall "foo" (<(tnat 1 \+ tnat 1)>).
-Example ex_reduce_tcall:
+Definition ex_tcall_tm := tcall "foo" (<(tnat 1 \+ tnat 1)>).
+Example ex_tcall:
   forall st,
-  ex_reduce_tcall_tm / st ==>* treturn (texec "foo") / push_call (trc (tnat 2) tvoid) st.
+  ex_tcall_tm / st ==>* treturn (texec "foo") / push_call (trc (tnat 2) tvoid) st.
 Proof.
-  unfold ex_reduce_tcall_tm. intros. simpl. repeat reduce. Qed.
+  unfold ex_tcall_tm. intros. simpl. repeat reduce. Qed.
 
-Definition ex_reduce_treturn_tm := treturn (tnat 1 \+ tnat 1).
-Example ex_reduce_treturn:
+Definition ex_treturn_tm := treturn (tnat 1 \+ tnat 1).
+Example ex_treturn:
   forall st,
-  ex_reduce_treturn_tm / st ==>* tnat 2 / pop_call st.
+  ex_treturn_tm / st ==>* tnat 2 / pop_call st.
 Proof.
-  unfold ex_reduce_treturn_tm. intros. repeat reduce. Qed.
+  unfold ex_treturn_tm. intros. repeat reduce. Qed.
 
-Definition ex_reduce_tcl_tm := tcl "foo" (<(tnat 1 \+ tnat 1)>).
-Example ex_reduce_tcl:
+Definition ex_tcl_tm := tcl "foo" (<(tnat 1 \+ tnat 1)>).
+Example ex_tcl:
   forall st,
-  ex_reduce_tcl_tm / st ==>* tcl "foo" (trc (tnat 2) tvoid) / st.
+  ex_tcl_tm / st ==>* tcl "foo" (trc (tnat 2) tvoid) / st.
 Proof.
-  unfold ex_reduce_tcl_tm. intros. repeat reduce. Qed.
+  unfold ex_tcl_tm. intros. repeat reduce. Qed.
 
-Definition ex_reduce_tnew_tm := tnew 2 "foo".
-Example ex_reduce_tnew:
-  ex_reduce_tnew_tm / init_state ==>* tref 1 / alloc_sr (tcl "foo" (<(tvoid, tvoid)>)) init_state.
+Definition ex_tnew_tm := tnew 2 "foo".
+Example ex_tnew:
+  ex_tnew_tm / init_state ==>* tref 1 / alloc_sr (tcl "foo" (<(tvoid, tvoid)>)) init_state.
 Proof.
-  unfold ex_reduce_tnew_tm. repeat reduce. Qed.
+  unfold ex_tnew_tm. repeat reduce. Qed.
 
-Definition ex_reduce_tfield_r_tm := (treturn (tref 1))@2.
-Example ex_reduce_tfield_r:
+Definition ex_tfield_r_tm := (treturn (tref 1))@2.
+Example ex_tfield_r:
   let st := push_call tvoid (alloc_sr (tcl "foo" (<(tvoid, tnat 1, tnat 2)>)) init_state) in
   let st' := pop_call st in
-  ex_reduce_tfield_r_tm / st ==>* tnat 2 / st'.
+  ex_tfield_r_tm / st ==>* tnat 2 / st'.
 Proof.
-  unfold ex_reduce_tfield_r_tm. repeat reduce. Qed.
+  unfold ex_tfield_r_tm. repeat reduce. Qed.
 
-Definition ex_reduce_tfield_w_tm := (treturn (tref 1)) <@ 1 <- (tnat 1 \+ tnat 1).
-Example ex_reduce_tfield_w:
+Definition ex_tfield_w_tm := (treturn (tref 1)) <@ 1 <- (tnat 1 \+ tnat 1).
+Example ex_tfield_w:
   let st := push_call tvoid (alloc_sr (tcl "foo" (<(tvoid, tvoid)>)) init_state) in
   let st' := write_sr 1 (tcl "foo" (<(tvoid, tnat 2)>)) (pop_call st) in
-  ex_reduce_tfield_w_tm / st ==>* tvoid / st'.
+  ex_tfield_w_tm / st ==>* tvoid / st'.
 Proof.
-  unfold ex_reduce_tfield_w_tm. repeat reduce. Qed.
+  unfold ex_tfield_w_tm. repeat reduce. Qed.
 
-Definition ex_reduce_tvnew_tm := tvnew 2 "foo".
-Example ex_reduce_tvnew:
+Definition ex_tvnew_tm := tvnew 2 "foo".
+Example ex_tvnew:
   forall st,
-  ex_reduce_tvnew_tm / st ==>* (tcl "foo" (<(tvoid, tvoid)>)) / st.
+  ex_tvnew_tm / st ==>* (tcl "foo" (<(tvoid, tvoid)>)) / st.
 Proof.
-  unfold ex_reduce_tvnew_tm. intros. repeat reduce. Qed.
+  unfold ex_tvnew_tm. intros. repeat reduce. Qed.
 
-Definition ex_reduce_tvfield_r_tm := tcl "foo" (<(tvoid, tnat 1, tnat 1 \+ tnat 1)>)?@2.
-Example ex_reduce_tvfield_r:
+Definition ex_tvfield_r_tm := tcl "foo" (<(tvoid, tnat 1, tnat 1 \+ tnat 1)>)?@2.
+Example ex_tvfield_r:
   forall st,
-  ex_reduce_tvfield_r_tm / st ==>* tnat 2 / st.
+  ex_tvfield_r_tm / st ==>* tnat 2 / st.
 Proof.
-  unfold ex_reduce_tvfield_r_tm. intros. repeat reduce. Qed.
+  unfold ex_tvfield_r_tm. intros. repeat reduce. Qed.
 
-Definition ex_reduce_tvfield_w_tm := (tvar 0) <?@ 1 <- (tnat 1 \+ tnat 1).
-Example ex_reduce_tvfield_w:
+Definition ex_tvfield_w_tm := (tvar 0) <?@ 1 <- (tnat 1 \+ tnat 1).
+Example ex_tvfield_w:
   let st := write_sk_hd 0 (tcl "foo" (<(tvoid, tvoid)>)) (resize_sk_hd 1 init_state) in
   let st' := write_sk_hd 0 (tcl "foo" (<(tvoid, tnat 2)>)) st in
-  ex_reduce_tvfield_w_tm / st ==>* tvoid / st'.
+  ex_tvfield_w_tm / st ==>* tvoid / st'.
 Proof.
-  unfold ex_reduce_tvfield_w_tm. repeat reduce. Qed.
+  unfold ex_tvfield_w_tm. repeat reduce. Qed.
 
 End Examples.
 
